We check the optimality conditions.
\begin{align*}
	0&=\Phi (\overline{u},0)+\Phi^*(u, \overline{p^*}) \\
	&= F(\overline{u})+G(A\overline{u})+F^*(A^*\overline{p^*})
	&= [F(\overline{u})+F^*(A^*\overline{p^*})-A^*\circ p^*(u)]+[G(A\overline{u})+G^*(-\overline{p^*})-(-p^*)(A\overline{u})]
\end{align*}

Using Young inequality $J(u)+J^*(u^*)-u^*(u)\geq 0$, $\forall u \in U$, and $\forall u^* \in U^*$, we see that both square brackets are nonnegative; and the sum is zero. Then
\begin{align*}
	F(\overline{u})+F^*(A^*\overline{p^*})=A^*\circ p^*(u) &\implies A^*p^* \in \partial F(\overline{u}) \\
	G(A\overline{u})+G^*(-\overline{p^*})=(-p^*)(A\overline{u}) &\implies -p^* \in \partial G(A\overleftarrow{u})
\end{align*}

$F$, $G$ are convex and locally bounded, one can show that 
$\sup\eqref{eq8. P*}=\inf\eqref{eq8. P}$.
\begin{example}[....Bounded variation]
	\begin{equation}
		J(u)=\frac{1}{2} \int_{\Omega}\abs{u(x)-v(x)}^2+\alpha \sup_{g\in C_0^\infty, \abs{g}\leq 1} \int_{\Omega} u dv g dx
	\end{equation}
	$\min_{u\in B(g)} J(u)$, $\mathcal{B}=\left\lbrace u\in L^1(\Omega) \ | \ V(u, \Omega) < \infty\right\rbrace$, where
	\begin{equation}
		V(u, \Omega)=\left\lbrace 
		\sup \int_{\Omega} u d_v g dx, g \in C_0^\infty (\Omega, \mathbb{R}^n), \norm{g}_\infty \leq 1
		\right\rbrace
	\end{equation}
	$\norm{u}_{BV}:= \norm{u}_{C^1(\Omega)}+V(u, \Omega)$,
	
	\begin{align*}
		\implies & F(u)=\frac{1}{2}\int_{\Omega} \abs{u(x)-v(x)}^2 dx = \norm{u-x}_{L^2(\Omega)}^2
	\end{align*}
	\[G(u)=\int_{\Omega} \abs{u}dx\]
	 where $A: \alpha \nabla$,
	\begin{align*}
		F^*(p^*)=\frac{1}{2} \int_{\Omega}\abs{p^*(x)-v(x)} ^2 -\frac{1}{2} v^2(x) dx
	\end{align*}
	and 
	\[G^*(p^*) =\left\lbrace 
	\begin{array}{cl}
		0, &\quad \abs{p^*} \leq 1 \\
	-\infty, &\quad \text{otherwise}
	\end{array}
	\right. \]
	
	$A^*=-\alpha \div$, therefore
	
	$J(p^*)=-\frac{1}{2} -\frac{1}{2} \int_{\Omega} -\alpha \div p^* + v^2+ \frac{1}{2} v^2 dx$
\end{example}

\subsection{Lagrangians}
\begin{definition}
	The function $L:U\times Y^* \rightarrow \overline{\mathbb{R}}$, $-L(u, p^*)=\sup_{p\in Y} \left\lbrace p^*(p) - \Phi(u, p)
	\right\rbrace$, is called Lagrangian or \eqref{eq8. P} relative to the perturbation $\Phi$. If we denote by $\Phi_u$ for fixed $u\in U$ the function $p\rightarrow \Phi(u, p)$, then $-L(u, p^*)=\Phi^*_u(p^*)$
\end{definition}

\begin{lemma}
	For all $u\in U$, the function $L_u: Y^* \rightarrow \overleftarrow{\mathbb{R}}$, $p^*\rightarrow L(u, p)$ is  a concave function (i.e. $-L_u$ is convex) and weak upper semi-continuous. If $\Phi$ is convex the for all $p^* \in Y^*$ the function $L_{p^*}: U\rightarrow \overline{\mathbb{R}}$, $u\rightarrow L(u, p^*)$ is convex.
	\begin{proof}
		Le valio verga otra vez. :@ 
	\end{proof}
\end{lemma}

Without assuming anything about $\Phi$, we obtain
\[
	\Phi^*(u^*, p^*) = \sup_{u\in U, p\in U} \left\lbrace u^*(u) + p^*(p) - 
	\right\rbrace
\]